coq/ZF/Meta/Decl/Axiom/Specification.v
@@ -1,0 +1,33 @@
+Require Import Coq.Lists.List.
+Require Import Coq.Strings.String.
+
+Require Import ZF.Meta.Env.
+Require Import ZF.Meta.Syntax.
+Require Import ZF.Meta.Term.Decl.
+Require Import ZF.Meta.Ty.
+
+Import ListNotations.
+
+(* forall P, forall a, exists b, forall x, x :< b <-> x :< a /\ P x             *)
+Definition Specification : DeclT :=
+  {| paraT := []
+  ;  resT  := TyProp
+  ;  bodyT :=
+      All VarTyClass
+        (All VarTySet
+          (Ex VarTySet
+            (All VarTySet
+              (Iff
+                (Elem (Var 0) (Var 1))
+                (And
+                  (Elem (Var 0) (Var 2))
+                  (App (Var 3) (Var 0)))))))
+  |}.
+
+Definition imports : Env := Env.empty.
+
+Definition exports : Env := Env.fromListT
+  [ ("Specification"%string, Specification)
+  ].
+
+Definition env : Env := Env.union imports exports.
